sme/Sme/ITree/Interp.lean
@@ -1,9 +1,41 @@
 import Sme.ITree.Defs
 import Sme.ITree.Bisim
 import Sme.ITree.Monad
+import Sme.ITree.Combinators
 
 namespace Sme.ITree
 
-def interp {M E : Type _ → Type _} (inp : ∀ X, E X → M X) : ∀ X, ITree E (PLift X) → M X :=
-  sorry
+universe u v w
+
+class Iter (M : Type u → Type _) where
+  iter {A B : Type u} : (A → M (A ⊕ B)) → A → M B
+
+instance {E : Type _ → Type _} : Iter (ITree E) where
+  iter := ITree.iter
+
+def interp {E : Type u → Type u} {M : Type (u + 1) → Type _}
+    [Monad M] [Iter M]
+    (inp : E ↝ (M ∘ PLift))
+    : ITree E ↝ M := fun _ v =>
+  Iter.iter (fun
+    | .ret x => pure <| .inr x
+    | .vis e k => (.inl ∘ ITree.dest ∘ k ∘ PLift.down) <$> inp _ e
+    | .tau x => pure <| .inl x.dest) v.dest
+
+inductive StateE (S : Type u) : Type u → Type u
+  | get : StateE S S
+  | put : S → StateE S PUnit
+
+instance {σ : Type u} {M : Type _ → Type _} [Iter M] [Functor M]
+    : Iter (StateT σ M) where
+  iter f a s := Iter.iter (fun ⟨a, s⟩ => (fun
+    | ⟨.inl x, y⟩ => .inl ⟨x, y⟩
+    | ⟨.inr x, y⟩ => .inr ⟨x, y⟩
+    ) <$> f a s) (Prod.mk a s)
+
+def StateE.handle {E} {S} : StateE S ↝ StateT S (ITree E) := fun
+  | _, .get => StateT.get
+  | _, .put v => StateT.set v
+
+end Sme.ITree
 
